Redo proof of load case for lower bound on registers formulation
Also optimized some parts of the old proof away, thanks to the new load spec

theories/ftlr/Load.v
@@ -71,42 +71,36 @@ Section fundamental.
   Qed.
 
   (* Description of what the resources are supposed to look like after opening the region if we need to, but before closing the region up again*)
-  Definition allow_load_res W r (regs : Reg) pc_a pc_p:=
+  Definition allow_load_res W r (regs : Reg) pc_a:=
     (∃ p g b e a, ⌜read_reg_inr regs r p g b e a⌝ ∗
-    if decide (reg_allows_load regs r p g b e a ) then
-       if decide (a ≠ pc_a) then
-         ∃ p' w, a ↦ₐ [p'] w  ∗ ⌜PermFlows p p'⌝ ∗ (region_open_resources W a [pc_a] p' interpC w false)
-       else ⌜PermFlows p pc_p⌝ ∗ open_region pc_a W
+    if decide (reg_allows_load regs r p g b e a ∧ a ≠ pc_a ) then
+         ∃ p' w, a ↦ₐ [p'] w  ∗ ⌜p' ≠ O⌝ ∗ (region_open_resources W a [pc_a] p' interpC w false)
       else open_region pc_a W)%I.
 
   Definition allow_load_mem W r (regs : Reg) pc_a pc_p pc_w (mem : PermMem) (bl: bool):=
     (∃ p g b e a, ⌜read_reg_inr regs r p g b e a⌝ ∗
-    if decide (reg_allows_load regs r p g b e a) then
-       if decide (a ≠ pc_a) then
+    if decide (reg_allows_load regs r p g b e a ∧ a ≠ pc_a) then
          ∃ p' w, ⌜mem = <[a:=(p',w)]> (<[pc_a:=(pc_p,pc_w)]> ∅)⌝ ∗
-            ⌜PermFlows p p'⌝ ∗ (region_open_resources W a [pc_a] p' interpC w bl)
-       else  ⌜mem = <[pc_a:=(pc_p,pc_w)]> ∅⌝ ∗ ⌜PermFlows p pc_p⌝ ∗ open_region pc_a W     else  ⌜mem = <[pc_a:=(pc_p,pc_w)]> ∅⌝ ∗ open_region pc_a W)%I.
+            ⌜p' ≠ O⌝ ∗ (region_open_resources W a [pc_a] p' interpC w bl)
+    else  ⌜mem = <[pc_a:=(pc_p,pc_w)]> ∅⌝ ∗ open_region pc_a W)%I.
 
   Lemma create_load_res:
     ∀ (W : leibnizO (STS * STS)) (r : leibnizO Reg) (p p' : Perm)
       (g : Locality) (b e a : Addr) (src : RegName) (p0 : Perm)
       (g0 : Locality) (b0 e0 a0 : Addr),
-      PermFlows p p'
-      → read_reg_inr (<[PC:=inr (p, g, b, e, a)]> r) src p0 g0 b0 e0 a0
+      read_reg_inr (<[PC:=inr (p, g, b, e, a)]> r) src p0 g0 b0 e0 a0
       → (∀ r1 : RegName, ⌜r1 ≠ PC⌝ → ((fixpoint interp1) W) (r !r! r1))
-          -∗ read_write_cond a p' interp
           -∗ open_region a W
           -∗ sts_full_world sts_std W
-          -∗ allow_load_res W src (<[PC:=inr (p, g, b, e, a)]> r) a p'
+          -∗ allow_load_res W src (<[PC:=inr (p, g, b, e, a)]> r) a
           ∗ sts_full_world sts_std W.
   Proof.
-    intros W r p p' g b e a src p0 g0 b0 e0 a0 Hpf HVsrc.
-    iIntros "#Hreg #Hinva Hr Hsts".
+    intros W r p p' g b e a src p0 g0 b0 e0 a0 HVsrc.
+    iIntros "#Hreg Hr Hsts".
     do 5 (iApply sep_exist_r; iExists _). iFrame "%".
-    destruct (decide (reg_allows_load (<[PC:=inr (p, g, b, e, a)]> r) src p0 g0 b0 e0 a0)). 1: rename r0 into Hallows.
+    case_decide. 1: destruct H3 as [Hallows Haeq].
     -  destruct Hallows as [Hrinr [Hra Hwb] ].
-       destruct (decide (a0 ≠ a)); rename n into Haeq.
-       * apply andb_prop in Hwb as [Hle Hge].
+         apply andb_prop in Hwb as [Hle Hge].
          rewrite /leb_addr in Hle,Hge.
 
          (* Unlike in the old proof, we now go the other way around, and prove that the source register could not have been the PC, since both addresses differ. This saves us some cases.*)
@@ -117,40 +111,25 @@ Section fundamental.
          rewrite /RegLocate Hrinr.
          iDestruct (read_allowed_inv _ a0 with "Hvsrc") as "Hconds"; auto;
            first (split; [by apply Z.leb_le | by apply Z.ltb_lt]).
-
          rewrite /read_write_cond.
          iDestruct "Hconds" as (p0' Hfl') "Hrel'".
+
          iDestruct (region_open_prepare with "Hr") as "Hr".
          iDestruct (readAllowed_valid_cap_implies with "Hvsrc") as "%"; eauto.
          { rewrite /withinBounds /leb_addr Hle Hge. auto. }
          destruct H3 as [Hregion' [ρ' [Hstd' Hnotrevoked'] ] ].
-         (*We can finally frame off Hsts here, since it is no longer needed after opening the region*)
+         (* We can finally frame off Hsts here, since it is no longer needed after opening the region*)
          iDestruct (region_open_next _ _ _ a0 p0' ρ' with "[$Hrel' $Hr $Hsts]") as (w0) "($ & Hstate' & Hr & Ha0 & % & Hfuture & #Hval)"; eauto.
          { apply not_elem_of_cons. split; auto. apply not_elem_of_nil. }
          iExists p0', w0. iSplitL "Ha0"; auto. iSplitR; auto. unfold region_open_resources.
          iExists ρ'. iFrame "%". iFrame. by iFrame "#".
-       * iFrame.
-         destruct (decide (src = PC)) ; simplify_eq.
-          + rewrite lookup_insert in Hrinr.
-            inversion Hrinr. rewrite -H4. auto.
-          +  iDestruct ("Hreg" $! src n) as "Hsrcv".
-              rewrite lookup_insert_ne in Hrinr; last by congruence.
-              rewrite /RegLocate Hrinr.
-              iDestruct (read_allowed_inv _ a0 with "Hsrcv") as (p'' Hfl') "#Harel'".
-              { apply andb_true_iff in Hwb as [Hle Hge].
-                split; [by apply Z.leb_le | by apply Z.ltb_lt]; auto. }
-              { destruct p0; inversion Hra; auto. }
-              rewrite /read_write_cond.
-              assert (a0 = a). by apply dec_stable.
-              rewrite -H3.
-                by iDestruct (rel_agree a0 p' p'' with "[$Hinva $Harel']") as "[-> _]".
-    - iFrame.
+        - iFrame.
   Qed.
 
   Lemma load_res_implies_mem_map:
     ∀ (W : leibnizO (STS * STS)) (r : leibnizO Reg) (p p' : Perm)
       (g : Locality) (b e a : Addr) (w : Word) (src : RegName),
-      allow_load_res W src (<[PC:=inr (p, g, b, e, a)]> r) a p'
+      allow_load_res W src (<[PC:=inr (p, g, b, e, a)]> r) a
       -∗ a ↦ₐ[p'] w
       -∗ ∃ mem0 : PermMem,
           allow_load_mem W src (<[PC:=inr (p, g, b, e, a)]> r) a p' w mem0 false
@@ -161,24 +140,17 @@ Section fundamental.
     iIntros "HLoadRes Ha".
     iDestruct "HLoadRes" as (p1 g1 b1 e1 a1) "[% HLoadRes]".
 
-    case_decide as Hallows.
+    case_decide as Hdec. 1: destruct Hdec as [ Hallows Haeq ].
     -  pose(Hallows' := Hallows). destruct Hallows' as [Hrinr [Hra Hwb] ].
-        case_decide as Haeq.
-        * iDestruct "HLoadRes" as (p'0 w0) "[HLoadCh HLoadRest]".
+          iDestruct "HLoadRes" as (p'0 w0) "[HLoadCh HLoadRest]".
           iExists _.
           iSplitL "HLoadRest".
           + iExists p1,g1,b1,e1,a1. iSplitR; first auto.
-            do 2 (case_decide; last by exfalso).
+            case_decide as Hdec1. 2: apply not_and_r in Hdec1 as [|]; by exfalso.
             iExists p'0,w0. iSplitR; auto.
           + iNext.
             iApply memMap_resource_2ne; auto; iFrame.
-      * iExists _.
-        iSplitL "HLoadRes".
-          + iExists p1,g1,b1,e1,a1. iSplitR; auto.
-            case_decide; last by exfalso. case_decide; first by exfalso.
-            iDestruct "HLoadRes" as (HPF) "HLoadRes". iSplitR; auto.
-          + iNext. by iApply memMap_resource_1.
-    - iExists _.
+        - iExists _.
       iSplitL "HLoadRes".
       + iExists p1,g1,b1,e1,a1. iSplitR; auto.
         case_decide; first by exfalso. auto.
@@ -189,30 +161,28 @@ Section fundamental.
     ∀ (W : leibnizO (STS * STS)) (r : leibnizO Reg) (p p' : Perm)
       (g : Locality) (b e a : Addr) (w : Word) (src : RegName)
       (mem0 : PermMem),
+        p' ≠ O →
         allow_load_mem W src (<[PC:=inr (p, g, b, e, a)]> r) a p' w mem0 false
         -∗ ⌜mem0 !! a = Some (p', w)⌝
           ∗ ⌜allow_load_map_or_true src (<[PC:=inr (p, g, b, e, a)]> r) mem0⌝.
   Proof.
-    iIntros (W r p p' g b e a w src mem0) "HLoadMem".
+    iIntros (W r p p' g b e a w src mem0 Hp'O) "HLoadMem".
     iDestruct "HLoadMem" as (p1 g1 b1 e1 a1) "[% HLoadRes]".
-    case_decide as Hallows.
+    case_decide as Hdec. 1: destruct Hdec as [ Hallows Haeq ].
     -  pose(Hallows' := Hallows). destruct Hallows' as [Hrinr [Hra Hwb] ].
-        case_decide as Haeq.
-        * iDestruct "HLoadRes" as (p'0 w0 ->) "[% _]".
+        (* case_decide as Haeq. *)
+          iDestruct "HLoadRes" as (p'0 w0 ->) "[% _]".
           iSplitR. rewrite lookup_insert_ne; auto. by rewrite lookup_insert.
           iExists p1,g1,b1,e1,a1. iSplitR; auto.
           case_decide; last by exfalso.
           iExists p'0,w0. iSplitR; auto.
           by rewrite lookup_insert.
-        * iDestruct "HLoadRes" as "[-> [% HLoadRes] ]".
+    - iDestruct "HLoadRes" as "[-> HLoadRes ]".
           iSplitR. by rewrite lookup_insert.
           iExists p1,g1,b1,e1,a1. iSplitR; auto.
-          case_decide; last by exfalso.
-          iExists p',w. by rewrite Haeq lookup_insert.
-    - iDestruct "HLoadRes" as "[-> HLoadRes]".
-      iSplitR. by rewrite lookup_insert.
-      iExists p1,g1,b1,e1,a1. iSplitR; auto.
-      case_decide; first by exfalso. auto.
+          case_decide as Hdec1; last by done.
+          apply not_and_r in Hdec as [|]; first by exfalso.
+          iExists p',w. apply dec_stable in H4 as <-. by rewrite lookup_insert.
   Qed.
 
   Lemma allow_load_mem_later:
@@ -226,12 +196,10 @@ Section fundamental.
     iDestruct "HLoadMem" as (p0 g0 b0 e0 a0) "[% HLoadMem]".
     do 5 (iApply later_exist_2; iExists _). iApply later_sep_2; iSplitR; auto.
     case_decide.
-    - case_decide.
       * iDestruct "HLoadMem" as (p'0 w0) "[-> [% HLoadMem] ]".
         do 2 (iApply later_exist_2; iExists _).
         do 2 (iApply later_sep_2; iSplitR; auto).
       * iFrame.
-    - iFrame.
   Qed.
 
   Lemma mem_map_recover_res:
@@ -249,23 +217,23 @@ Section fundamental.
     intros W r p p' g b e a w src p0 p'0 g0 b0 e0 a0 mem0 loadv Hrar Ha0.
     iIntros "HLoadMem #Hw Hmem".
     iDestruct "HLoadMem" as (p1 g1 b1 e1 a1) "[% HLoadRes]".
-    destruct (decide (reg_allows_load (<[PC:=inr (p, g, b, e, a)]> r) src p1 g1 b1 e1 a1)). 1: rename r0 into Hallows.
+    case_decide as Hdec. destruct Hdec as [Hallows Heq].
     -  destruct Hallows as [Hrinr [Hra Hwb] ].
-        destruct (decide (a1 ≠ a)); rename n into Haeq.
-        * iDestruct "HLoadRes" as (p'1 w0) "[-> [% HLoadRes] ]".
-          iDestruct "HLoadRes" as (ρ1) "(Hstate' & % & Hr & % & (Hfuture & #HV) & Hrel')".
-          rewrite -memMap_resource_2ne. iDestruct "Hmem" as  "[Ha1 $]".
-          iDestruct (region_close_next with "[$Hr $Ha1 $Hrel' $Hstate' $Hfuture]") as "Hr"; eauto.
-          { apply not_elem_of_cons; split; [auto|apply not_elem_of_nil]. }
-          iDestruct (region_open_prepare with "Hr") as "$".
-          destruct (load_inr_eq Hrar H3) as (<- & <- &<- &<- &<-).
-          rewrite lookup_insert in Ha0; inversion Ha0. all: done.
-        * apply dec_stable in Haeq.
-          iDestruct "HLoadRes" as "[-> [% $ ] ]".
-          rewrite -memMap_resource_1.
-          destruct (load_inr_eq Hrar H3) as (<- & <- &<- &<- &<-).
-          rewrite Haeq lookup_insert in Ha0. inversion Ha0. by iFrame.
-    - destruct (load_inr_eq Hrar H3) as (<- & <- &<- &<- &<-); by exfalso.
+       iDestruct "HLoadRes" as (p'1 w0) "[-> [% HLoadRes] ]".
+       iDestruct "HLoadRes" as (ρ1) "(Hstate' & % & Hr & % & (Hfuture & #HV) & Hrel')".
+       rewrite memMap_resource_2ne; last auto. iDestruct "Hmem" as  "[Ha1 $]".
+       iDestruct (region_close_next with "[$Hr $Ha1 $Hrel' $Hstate' $Hfuture]") as "Hr"; eauto.
+       { apply not_elem_of_cons; split; [auto|apply not_elem_of_nil]. }
+       iDestruct (region_open_prepare with "Hr") as "$".
+       destruct (load_inr_eq Hrar H3) as (<- & <- &<- &<- &<-).
+       rewrite lookup_insert in Ha0; inversion Ha0. all: done.
+    - apply not_and_r in Hdec as [|].
+      * destruct (load_inr_eq Hrar H3) as (<- & <- &<- &<- &<-); by exfalso.
+      * apply dec_stable in H4 as <-.
+        iDestruct "HLoadRes" as "[-> $ ]".
+        rewrite -memMap_resource_1.
+        destruct (load_inr_eq Hrar H3) as (<- & <- &<- &<- &<-).
+        rewrite lookup_insert in Ha0. inversion Ha0. by iFrame.
   Qed.
 
 
@@ -298,7 +266,7 @@ Section fundamental.
     }
 
     (* Step 1: open the region, if necessary, and store all the resources obtained from the region in allow_load_res *)
-    iDestruct (create_load_res with "Hreg Hinva Hr Hsts") as "[HLoadRes Hsts]"; eauto.
+    iDestruct (create_load_res with "Hreg Hr Hsts") as "[HLoadRes Hsts]"; eauto.
     (* Clear helper values; they exist in the existential now *)
     clear HVsrc p0 g0 b0 e0 a0.
 
@@ -306,13 +274,15 @@ Section fundamental.
     iDestruct (load_res_implies_mem_map W  with "HLoadRes Ha") as (mem) "[HLoadMem HMemRes]".
 
     (* Step 3:  derive the non-spatial conditions over the memory map*)
-    iDestruct (mem_map_implies_pure_conds with "HLoadMem") as %(HReadPC & HLoadAP).
+    iDestruct (mem_map_implies_pure_conds with "HLoadMem") as %(HReadPC & HLoadAP); auto.
 
     (* Step 4: move the later outside, so that we can remove it after applying wp_load *)
     iDestruct (allow_load_mem_later with "HLoadMem") as "HLoadMem".
 
     iApply (wp_load with "[Hmap HMemRes]"); eauto.
     {by rewrite lookup_insert. }
+    { rewrite /subseteq /map_subseteq /set_subseteq. intros rr _.
+      apply elem_of_gmap_dom. rewrite lookup_insert_is_Some'; eauto. }
     {iSplitR "Hmap"; auto. }
     iNext. iIntros (regs' retv). iDestruct 1 as (HSpec) "[Hmem Hmap]".
 
